coq/JsInterpreter.v
@@ -745,6 +745,11 @@ Definition to_default (run_call' : run_call_type) S C l (prefo : option preftype
       let lf := value_object lfo in
       match run_callable S lf with
       | Some fc =>
+        (* We burden from the beginning to the end those [run_call']
+        attributes, while we could burden only [call'] attributes
+        which seems lighter and clearer, all hat because of the next
+        line (which could actually be replaced by a [call], but would
+        it be clearer to add such a deferencing?) *)
         if_success_value run_call' C (run_call' S C fc (Some lfo) (Some lf) nil) (fun S2 v =>
           match v with
           | value_prim w => out_ter S w
